src/mapping/PStoRMWUtils.v
@@ -18,13 +18,13 @@ From PromisingIR Require Import Time.
 From PromisingIR Require Import View.
 From PromisingIR Require Import BoolMap.
 From PromisingIR Require Import Promises.
-From PromisingIR Require Import Reserves.
 From PromisingIR Require Import Cell.
 From PromisingIR Require Import Memory.
 From PromisingIR Require Import TView.
 From PromisingIR Require Import Global.
 From PromisingIR Require Import Local.
 From PromisingIR Require Import Thread.
+From PromisingIR Require Import Configuration.
 
 Require Import PromisingArch.lib.Basic.
 Require Import PromisingArch.lib.Order.
@@ -42,9 +42,16 @@ Module PSLoc := PromisingLib.Loc.Loc.
 Module PSTime := PromisingIR.Time.Time.
 Module PSView := PromisingIR.View.View.
 Module PSPromises := PromisingIR.Promises.Promises.
+Module PSTView := PromisingIR.TView.TView.
 Module PSLocal := PromisingIR.Local.Local.
+Module PSCell := PromisingIR.Cell.Cell.
 Module PSMemory := PromisingIR.Memory.Memory.
+Module PSGlobal := PromisingIR.Global.Global.
+Module PSThread := PromisingIR.Thread.Thread.
+Module PSConfiguration := PromisingIR.Configuration.Configuration.
 
+
+(* timestamp conversion between PS and ARM *)
 
 Fixpoint ntt (n: nat): PSTime.t :=
   match n with
@@ -98,3 +105,21 @@ Proof.
   - apply ntt_le. rewrite EQ. refl.
   - apply ntt_le. rewrite EQ. refl.
 Qed.
+
+
+(* SC fence with sc view le n *)
+
+Section DMBSY.
+  Context `{A: Type, _: orderC A eq}.
+
+  Lemma dmbsy_le_cases
+        n tid eu1 eu4
+        (STEPS: rtc (RMWExecUnit.state_step_dmbsy_over n tid) eu1 eu4):
+    (<<STEPS_DMBSY: rtc (RMWExecUnit.state_step_dmbsy_over (S n) tid) eu1 eu4>>) \/
+    exists eu2 eu3,
+      (<<STEPS_DMBSY1: rtc (RMWExecUnit.state_step_dmbsy_exact n tid) eu1 eu2>>) /\
+      (<<STEP_DMBSY: RMWExecUnit.state_step_dmbsy n tid eu2 eu3>>) /\
+      (<<STEPS_DMBSY2: rtc (RMWExecUnit.state_step_dmbsy_over (S n) tid) eu3 eu4>>).
+  Proof.
+  Admitted.
+End DMBSY.
